Outline the core simplification theorems

src/tools/symbexec/symb_rulesScript.sml
@@ -664,7 +664,7 @@ val symb_rule_FRESH_thm = store_thm(
 (*        RULE SUBST         *)
 (* ************************* *)
 val symb_simplification_def = Define `
-  symb_simplification sr sys symbexp symbexp' =
+    symb_simplification sr sys symbexp symbexp' =
     (!H.
        (symb_interpr_welltyped sr H) ==>
        (symb_interpr_for_symbs
@@ -676,6 +676,144 @@ val symb_simplification_def = Define `
        (sr.sr_interpret_f H symbexp = sr.sr_interpret_f H symbexp')
     )
 `;
+
+val symb_simplification_e_def = Define `
+    symb_simplification_e sr pcond symbexp symbexp' =
+    (!H.
+       (symb_interpr_welltyped sr H) ==>
+       (symb_interpr_for_symbs
+            ((sr.sr_symbols_f pcond) UNION
+             (sr.sr_symbols_f symbexp) UNION
+             (sr.sr_symbols_f symbexp')) H) ==>
+
+       (sr.sr_interpret_f H pcond = SOME sr.sr_val_true) ==>
+       (sr.sr_interpret_f H symbexp = sr.sr_interpret_f H symbexp')
+    )
+`;
+
+val symb_simplification_thm = store_thm(
+   "symb_simplification_thm", ``
+!sr.
+!sys symbexp symbexp'.
+  (symb_simplification sr sys symbexp symbexp') ==>
+  (symb_simplification_e sr (symb_symbst_pcond sys) symbexp symbexp')
+``,
+  METIS_TAC [symb_simplification_def, symb_simplification_e_def, symb_interpr_symbpcond_def]
+);
+
+val symb_exp_imp_def = Define `
+    symb_exp_imp sr pcond pcond' =
+    ((sr.sr_symbols_f pcond' SUBSET sr.sr_symbols_f pcond) /\
+     (!H.
+       (symb_interpr_welltyped sr H) ==>
+       (symb_interpr_for_symbs
+            (sr.sr_symbols_f pcond) H) ==>
+
+       (sr.sr_interpret_f H pcond  = SOME sr.sr_val_true) ==>
+       (sr.sr_interpret_f H pcond' = SOME sr.sr_val_true)
+     )
+    )
+`;
+
+val symb_simplification_IMP_thm = store_thm(
+   "symb_simplification_IMP_thm", ``
+!sr.
+!pcond pcond' symbexp symbexp'.
+  (symb_exp_imp sr pcond pcond') ==>
+  (symb_simplification_e sr pcond' symbexp symbexp') ==>
+  (symb_simplification_e sr pcond  symbexp symbexp')
+``,
+  cheat
+);
+
+val symb_simplification_UnsignedCast_thm = store_thm(
+   "symb_simplification_UnsignedCast_thm", ``
+!sr.
+!pcond symbexp symbexp' sz.
+  (symb_simplification_e sr pcond symbexp symbexp') ==>
+  (symb_simplification_e sr pcond (BExp_Cast BIExp_UnsignedCast symbexp sz) (BExp_Cast BIExp_UnsignedCast symbexp' sz))
+``,
+  cheat
+);
+
+val symb_simplification_IfThenElse_T_thm = store_thm(
+   "symb_simplification_IfThenElse_T_thm", ``
+!sr.
+!pcond ec et ef.
+  (symb_simplification_e sr ec (BExp_IfThenElse ec et ef) et)
+``,
+  cheat
+);
+
+val symb_simplification_IfThenElse_F_thm = store_thm(
+   "symb_simplification_IfThenElse_F_thm", ``
+!sr.
+!pcond ec et ef.
+  (symb_simplification_e sr (BExp_UnaryExp BIExp_Not ec) (BExp_IfThenElse ec et ef) ef)
+``,
+  cheat
+);
+
+(* TODO: need to typecheck the whole expression, also in the next theorem *)
+val symb_simplification_Mem_Match_thm = store_thm(
+   "symb_simplification_Mem_Match_thm", ``
+!sr.
+!be_m be_sa be_v be_la sz masz mvsz.
+  (type_of_bir_exp be_m = SOME (BType_Mem masz mvsz)) ==>
+  (type_of_bir_exp be_v = SOME (BType_Imm sz)) ==>
+  (symb_simplification_e sr
+    (BExp_BinPred BIExp_Equal be_la be_sa)
+    (BExp_Load
+      (BExp_Store
+        be_m
+        be_sa
+        BEnd_LittleEndian
+        be_v)
+      be_la
+      BEnd_LittleEndian
+      sz)
+    (be_v)
+  )
+``,
+  cheat
+);
+
+(* TODO: corner cases? make it so it also works for these *)
+(* TODO: need one of these for 32bit stores as well, and the other two combinations *)
+val symb_simplification_Mem_Bypass_thm = store_thm(
+   "symb_simplification_Mem_Bypass_thm", ``
+!sr.
+!be_m be_sa be_v be_la.
+  (type_of_bir_exp be_m = SOME (BType_Mem Bit32 Bit8)) ==>
+  (type_of_bir_exp be_v = SOME (BType_Imm Bit8)) ==>
+  (symb_simplification_e sr
+    (BExp_BinExp BIExp_Or
+       (BExp_BinPred BIExp_LessOrEqual
+         (BExp_BinExp BIExp_Plus be_la (BExp_Const (Imm32 4w)))
+         be_sa)
+       (BExp_BinPred BIExp_LessOrEqual
+         (BExp_BinExp BIExp_Plus be_sa (BExp_Const (Imm32 1w)))
+         be_la))
+    (BExp_Load
+      (BExp_Store
+        be_m
+        be_sa
+        BEnd_LittleEndian
+        be_v)
+      be_la
+      BEnd_LittleEndian
+      Bit32)
+    (BExp_Load
+      be_m
+      be_la
+      BEnd_LittleEndian
+      Bit32)
+  )
+``,
+  cheat
+);
+
+
 
 val symb_simplification_matchstate_IMP_matchstate_thm = store_thm(
    "symb_simplification_matchstate_IMP_matchstate_thm", ``
